src/Variables.v
@@ -1,0 +1,118 @@
+Require Import Hlist.
+Require Import List.
+Require Import PeanoNat.
+
+Set Implicit Arguments.
+
+Definition var contents (t:Type) : Type := @member Type t contents.
+
+(* A list of variables whose types are drawn from contents and which
+have types vartypes (which must be a subset of contents for a list of
+variables to be well-typed). *)
+Definition variables contents vartypes :=
+  hlist (var contents) vartypes.
+
+(* version of member_index suitable for use in hmap; contents is made
+   implicit and maximally inserted so var_index has the intended
+   meaning as a partially applied function. *)
+Definition var_index {contents} := fun t (m:var contents t) => member_index m.
+
+Lemma var_type_in : forall contents t,
+    var contents t ->
+    In t contents.
+Proof.
+  induction 1; eauto using in_eq, in_cons.
+Qed.
+
+(* Proof of the above remark that vartypes must be a subset of contents. *)
+Remark variables_property : forall contents vartypes,
+    variables contents vartypes ->
+    (forall t, In t vartypes -> In t contents).
+Proof.
+  induction contents; intros.
+  - inversion X; subst.
+    inversion H.
+    inversion X0; subst.
+  - induction X; subst.
+    inversion H.
+    inversion H; subst; eauto using var_type_in.
+Qed.
+
+Theorem hin_index_vars : forall contents t (m: var contents t)
+                           typevars (vars: variables contents typevars),
+    HIn m vars <->
+    In (member_index m) (hmap var_index vars).
+Proof.
+  apply hin_iff_index_in.
+Qed.
+
+Theorem member_index_eq_var_index : forall contents t
+  (m: member t contents),
+  member_index m = var_index m.
+Proof. reflexivity. Qed.
+
+Section Modification.
+
+  Definition modified contents vartypes
+             (vars: hlist (fun T:Type => var contents T) vartypes)
+             (l l': hlist (fun T:Type => T) contents) : Prop :=
+    forall t (m:var contents t), (HIn m vars -> False) ->
+                            get m l = get m l'.
+
+  Theorem NoDup_get_neq : forall A (def:A) (l:list A) n1 n2,
+      n1 < length l ->
+      n2 < length l ->
+      n1 <> n2 ->
+      NoDup l ->
+      nth n1 l def <> nth n2 l def.
+  Proof.
+    intros.
+    contradict H1.
+    eapply NoDup_nth; eauto.
+  Qed.
+
+  Ltac distinguish_indices :=
+    match goal with
+    | [ |- member_index ?m <> member_index ?m' ] =>
+      case_eq (Nat.eq_dec (member_index m') (member_index m)); intros; auto;
+      exfalso;
+      match goal with
+      | [ H: member_index m' = member_index m |- _ ] =>
+        rewrite H in *; clear H
+      end
+    end.
+
+  Lemma hin_get_variables : forall contents vartypes
+                              (vars: variables contents vartypes)
+                              t (v: var vartypes t),
+      HIn (get v vars) vars.
+  Proof.
+    apply hin_get.
+  Qed.
+
+  Lemma modified_nothing : forall contents vartypes
+                             (vars: variables contents vartypes)
+                             (m: hlist (fun T:Type => T) contents),
+      modified vars m m.
+  Proof.
+    unfold modified; intros; auto.
+  Qed.
+
+  Hint Resolve hin_get_variables.
+  Hint Resolve -> hin_index_vars.
+  Hint Resolve <- hin_index_vars.
+
+  Lemma one_more_modified : forall contents vartypes
+                              (vars: variables contents vartypes)
+                              t v (val': t)
+                              (m m': hlist (fun T:Type => T) contents),
+      modified vars m m' ->
+      modified vars m (set (get v vars) val' m').
+  Proof.
+    unfold modified; intros.
+    rewrite hin_index_vars in H0.
+    rewrite get_set_other; eauto.
+    distinguish_indices; auto.
+  Qed.
+
+End Modification.
